\documentclass{article}
\setlength\parindent{0pt}
\setlength{\parskip}{0pt}
\usepackage{amsmath}
\usepackage{mathtools}
\usepackage{amssymb}
\usepackage[linesnumbered,boxed]{algorithm2e}
\SetKwInput{KwInput}{Input}
\SetKwInput{KwOutput}{Output}
\SetKwInput{KwInt}{Initialize}
\usepackage{mathrsfs}
\usepackage{tcolorbox}
\usepackage{float}
\usepackage{geometry}
\geometry{a4paper,scale=0.8}
\usepackage{graphicx}
\usepackage{setspace}
\usepackage{enumitem}
\usepackage{ulem}
\linespread{1.5}
\newcommand{\indep}{\rotatebox[origin=c]{90}{$\models$}}


\begin{document}

\title{Title}

\author{Author}

\maketitle

\section{PDF CDF and Survival Function}

\begin{equation}
	h(t) = \frac{f(t)}{S(t)}
\end{equation}

\begin{equation}
	f(x) = PDF \quad F(x) = CDF \quad S(x) = 1 - F(x) 
\end{equation}

\begin{equation}
	F(x) = \sum_{i=1}^t P(X = t)
\end{equation}

\begin{align}
	P(X = 1) = \frac{1}{6}\\
	P(X = 2) = \frac{1}{6}\\
	P(X = 3) = \frac{1}{6}\\
	P(X = 4) = \frac{1}{6}\\
	P(X = 5) = \frac{1}{6}\\
	P(X = 6) = \frac{1}{6}
\end{align}

\begin{align}
	F(X = 1) = \frac{1}{6} \\
	F(X = 2) = \frac{2}{6} \\
	F(X = 3) = \frac{3}{6} \\
	F(X = 4) = \frac{4}{6} \\
	F(X = 5) = \frac{5}{6} \\
	F(X = 6) = 1
\end{align}

\begin{equation}
	F(x) = \int_{-\infty}^x  f(t) dt
\end{equation}

\begin{equation}
	Y = X \beta + \epsilon 
\end{equation}

\begin{equation}
	\begin{pmatrix}
		y_1 \\ \vdots \\ y_n
	\end{pmatrix} = 
	\begin{pmatrix}
		x_{11} & \ldots & x_{p1} \\ \vdots & \ddots & \vdots \\ x_{1n} & \ldots & x_{pn} 
	\end{pmatrix}^T \times
	\begin{pmatrix}
		\beta_1 \\ \vdots \\ \beta_p
	\end{pmatrix} + 
	\begin{pmatrix}
		\epsilon_1 \\ \vdots \\ \epsilon_n
	\end{pmatrix}
\end{equation}


\begin{equation}
	y_1 = x_{11} \times \beta_{11} + x_{12} \times \beta_2 \ldots  x_{p1} \times \beta_p + \epsilon_1 = \sum_{i=1} ^ p \beta_i\times x_{i1} + \epsilon_1
\end{equation}

\begin{align}
	h(t) &= h_0(t) \times e^{X\beta + \epsilon} \\
	& = h_0(t) \times e^{X\beta} \times e^\epsilon   \quad\quad e^{a+b} = e^a \times e^b  \\
	& = h_0'(t) \times  e^{X\beta} \quad\quad h_0'(t) = h_0(t) e^{\epsilon}\\
	\frac{h(t)}{h_0'(t)} &= e^{X\beta}\\
	\ln \Bigg( \frac{h(t)}{h_0'(t)} \Bigg) & = \ln e^{X\beta} = X\beta \quad\quad log_e^{e^a} = a
\end{align}
	
















\end{document}
